<?xml version="1.0" encoding="UTF-8"?>

<section xml:id="sec-pol_cord" xmlns:xi="http://www.w3.org/2001/XInclude">
  <title>Polar Coordinate</title>

  <image source ="polarCord.png" width="60%"> </image>
  
  <p> Here, <m>\hat{r}=\hat{r}(\theta)</m> </p>
  <men xml:id="eqn-polar1">
    \hat{r} = \hat{x}\cos\theta + \hat{y}\sin\theta
  </men>
  <p>
    and 
    <me>
      \frac{\,d\hat{r}}{\,d\theta}=-\hat{x}\sin\theta + \hat{y}\cos\theta
    </me>
    Now 
   <me>\hat{r} \cdot \frac{d\hat{r}}{d\theta} =0 </me> 
 <m>
  \Rightarrow \hat{r} 
 </m>
  is perpendicular on <m>\frac{d\hat{r}}{d\theta}.</m>
 
  </p>

  <p>
    Therefore, we call 
    <men xml:id="eqn-polar2">
      \frac{\,d\hat{r}}{\,d\theta}=-\hat{x}\sin\theta + \hat{y}\cos\theta =\hat{\theta}
    </men>
  </p>
  <p> Also, <m>\hat{\theta}=\hat{\theta}(\theta)</m> </p>

  <p>
    and, 
    <men xml:id="eqn-polar3">
      \frac{\,d\hat{\theta}}{\,d\theta}=-\hat{x}\cos\theta - \hat{y}\sin\theta =-\hat{r}
    </men>
  </p>
  
  <p>
    Now, 
    <md>
      <mrow> \vec{v}\amp  = \frac{\,d\vec{r}}{\,dt}</mrow>
      <mrow> \amp  = \frac{\,d}{\,dt}(r\hat{r}) </mrow>
      <mrow> \amp =\dot{r}\hat{r} + r \frac{\,d\hat{r}}{\,dt}</mrow>
      <mrow> \amp =\dot{r} \hat{r} + r \frac{\,d\hat{r}}{\,d\theta} \frac{\,d\theta}{\,dt} </mrow>
    </md>

<m>\because \theta =\theta(t)</m>

    <men xml:id="eqn-polar4">
      \therefore \vec{v} = \dot{r} \hat{r} +r\dot{\theta}\hat{\theta} = v_r +v_{\theta}
    </men>
  </p>

  <p>
    Again, 
    <md>
      <mrow> \vec{a}\amp =\frac{\,d\vec{v}}{\,dt} </mrow>
      <mrow> \amp = \frac{\,d}{\,dt}( \dot{r} \hat{r} +r\dot{\theta}\hat{\theta}) </mrow>
      <mrow> \amp =\ddot{r} \hat{r} +\dot{r}\frac{\,d\hat{r}}{\,dt} + \dot{r}\dot{\theta}\hat{\theta} + r\ddot{\theta}\hat{\theta} + r\dot{\theta}\frac{\,d\hat{\theta}}{\,dt}</mrow>
      <mrow> \amp =  \ddot{r} \hat{r} +\dot{r}\frac{\,d\hat{r}}{\,d\theta} \frac{\,d\theta}{\,dt} 
        + \dot{r}\dot{\theta}\hat{\theta} +  r\ddot{\theta}\hat{\theta} + r\dot{\theta}\frac{\,d\hat{\theta}}{\,d\theta} \frac{\,d\theta}{\,dt}
      </mrow>
      <mrow> \amp = \ddot{r} \hat{r} + 2\dot{r}\dot{\theta}\hat{\theta}+r\ddot{\theta}\hat{\theta}-r\dot{\theta}^2\hat{r} </mrow>
    </md>

    
    <men xml:id="eqn-polar5">
      \therefore \vec{a} = (\ddot{r} -r\dot{\theta}^2)\hat{r} + (2\dot{r}\dot{\theta}+r\ddot{\theta})\hat{\theta} = a_r +a_{\theta}
    </men>

  </p>

</section>