<?xml version="1.0" encoding="UTF-8"?>

<section xml:id="sec-kepI_law" xmlns:xi="http://www.w3.org/2001/XInclude">
  <title>Derivation of Kepler's I Law</title>
<introduction>
 
  <image source ="ellipse.png" width="70%"> </image>

  <p> From Newton's Law of Gravitation and Newton's II law of motion. </p>
  <p>
    
 
<men xml:id="eqn-newt1">
  \vec{F} = -\frac{GMm}{r^2}\hat{r}
</men>

<men xml:id="eqn-newt2">
  \vec{F} =m\vec{a_r}
</men>

Using <xref ref="eqn-polar5"/>
<me>
or, \quad  m (\ddot{r} -r\dot{\theta}^2)\hat{r} = -\frac{GMm}{r^2}\hat{r}
</me>

<men xml:id="eqn-newt3">
  \ddot{r} -r\dot{\theta}^2 = -\frac{GM}{r^2}
</men>
From principle of conservation of angular momentum:

<md>
  <mrow> L \amp = \vec{r}\times\vec{p}</mrow>
  <mrow>  \amp = m(\vec{r}\times\vec{v})</mrow>
  <mrow> \amp = m[\vec{r}\times(\dot{r}\hat{r}+r\dot{\theta}\hat{\theta})] </mrow>
  <mrow> \amp = m(r^2\dot{\theta})</mrow>
</md>

using <xref ref="eqn-polar4"/> and <m>\quad \because  \hat{r}\times\hat{\theta} = \sin(90)=1 \quad </m> and <m>\quad \hat{r}\times\hat{r} = \sin(0)=0</m>
<men xml:id="eqn-newt4">
  \therefore \dot{\theta} = \frac{L}{mr^2}
</men>
For convenience let's say 
<men xml:id="eqn-newt5">
  \frac{L}{m}=h
</men>
Also to solve <xref ref="eqn-newt3"/> we need to change the variable <m>r</m> to its inverse,  
<men xml:id="eqn-newt6">
  \frac{1}{r}=u
</men>
 and then change the variable <m>t</m> to  <m>\theta</m>. This mathematical trick was adopted by 
 <alert>Bernaulli</alert> to solve differential equation of variable coefficient such as
 <me>
  \frac{dy}{dx}+p(x)y=q(x)y^n
 </me>
 here <m>u=y^{(1-n)}</m>. In <xref ref="eqn-newt3"/> <m>n=2</m> as power of <m>r.</m>
</p>

<p>
  Hence, differentiate <xref ref="eqn-newt6"/> with respect to <m>'t'.</m>
  <md>
    <mrow> -\frac{1}{r^2}\frac{\,dr}{\,dt} \amp = \frac{\,du}{\,dt} </mrow>
    <mrow> \amp =\frac{\,du}{\,d\theta} \frac{\,d\theta}{\,dt} \quad \text{(chain rule)}</mrow>
    <mrow>or, \quad \dot{r} \amp =-\frac{1}{u^2}\dot{\theta}\frac{\,du}{\,d\theta} </mrow>
  </md>

  <men xml:id="eqn-newt7">
    \therefore \quad \dot{r} = -h\frac{\,du}{\,d\theta}
  </men>

  from <xref ref="eqn-newt4"/>, <xref ref="eqn-newt5"/> and <xref ref="eqn-newt6"/>, we have 
  <men xml:id="eqn-newt8">
    \dot{\theta}= \frac{L}{mr^2}=hu^2
  </men>
  
  Differentiate <xref ref="eqn-newt7"/> w.r. t. <m>'t'</m> again, we get -
  <md>
    <mrow>\ddot{r} \amp =-h\frac{\,d}{\,dt}(\frac{\,du}{\,d\theta}) </mrow>
    <mrow> \amp =-h\frac{\,d}{\,d\theta}(\frac{\,du}{\,d\theta})\frac{\,d\theta}{\,dt}</mrow>
    <mrow> \amp =-h\dot{\theta}\frac{\,d^2 u}{\,d\theta^2}</mrow>
  </md>

  <men xml:id="eqn-newt9">
    \therefore \quad \ddot{r} =-h^2u^2\frac{\,d^2 u}{\,d\theta^2}
  </men>
  

</p>


<p>
  
  From <xref ref="eqn-newt3"/>
  <me>
    -h^2u^2\frac{\,d^2 u}{\,d\theta^2} - \frac{1}{u}(h^2u^4)=-GMu^2
  </me>
  
  <me>
    or,\quad \frac{\,d^2 u}{\,d\theta^2} +u =\frac{GM}{h^2} =\frac{k}{h^2} \quad (say)
  </me>
  
  assume <m>k=GM</m>

  <me>
    or, \quad \frac{\,d^2}{\,d\theta^2} (u-\frac{k}{h^2}) +  (u-\frac{k}{h^2}) =0
  </me>

  Again say, 
  <men xml:id="eqn-newt10">
    u-\frac{k}{h^2} = y
  </men>
  
  <men xml:id="eqn-newt11">
    \therefore \quad \frac{\,d^2 y}{\,d\theta^2}+y =0
  </men>
  This is homogeneous second order linear differential equation with constant coefficient. The solution of which can be given as 

  <men xml:id="eqn-newt12">
    y = A\cos\theta
  </men>
  
where <m>A</m> is an arbitrary constant whose value can be determined by initial condition. There are other possible solution to this equation as well 
such as <m>y=A\cos\theta+B\sin\theta </m> or simply <m>y =B\sin\theta.</m>

 <md>
  <mrow>  or, \quad u - \frac{k}{h^2} \amp = A\cos\theta</mrow>
  <mrow> u \amp =\frac{k}{h^2}+A\cos\theta </mrow>
  <mrow> \amp = \frac{k}{h^2}[1+\frac{Ah^2}{k}\cos\theta] </mrow>
  <mrow> \amp = \frac{k}{h^2}[1+e\cos\theta]</mrow>
 </md>
  
  <me>
    or,\quad \frac{1}{r}=\frac{k}{h^2}[1+e\cos\theta]
  </me>
  <me>
    or,\quad r = \frac{h^2}{k}[\frac{1}{1+e\cos\theta}]
  </me>
  
<men xml:id="eqn-newt13">
  \therefore \quad r=\frac{l}{1+e\cos\theta}
</men>

  The <xref ref="eqn-newt13"/> is equation of conic section, where <m>e=0,</m> represents circle, <m>0\lt e \lt 1</m> represents ellipse, <m>e=1,</m>
is parabola, and <m>e\gt 1 </m> represents hyperbola.

In <xref ref="eqn-newt13"/>
 <men xml:id="eqn-newt14">
  e = \frac{Ah^2}{k} = \frac{AL^2}{GMm^2} = eccentricity.
</men>
and 

<men xml:id="eqn-newt15">
  l = \frac{h^2}{k} =\frac{L^2}{GMm^2}=\quad \text{semi-latus rectum}
</men>

</p>
<p>
  If <xref ref="eqn-newt13"/> is an equation of ellipse then
  <me>
    e = \sqrt{1-\frac{b^2}{a^2}}
  </me>
  So let's prove it.
</p>
  <proof>
    <p>
    In ellipse semi-major axis <m>a</m> is the arithmatic mean of <m>r_{max}</m> and <m>r_{min}</m>.
  <me>
    \therefore \quad a=\frac{1}{2}[r_{max}+r_{min}] = \frac{1}{2}[\frac{l}{1-e}+\frac{l}{1+e}] 
  </me>
  At <m>\theta = 0</m> and <m>\pi</m> from <xref ref="eqn-newt13"/>.
  <men xml:id="eqn-newt16">
    \therefore \quad a = \frac{l}{1-e^2}
  </men>
  also semi-minor axis <m>b</m> is a geometric mean of <m>r_{max}</m> and <m>r_{min}</m>.
  <men xml:id="eqn-newt17">
    \therefore \quad b^2 = r_{max}r_{min} =  \frac{l^2}{1-e^2}
  </men>

  <me>
    or,\quad b^2 =  \frac{l^2(1-e^2)}{(1-e^2)^2} = a^2(1-e^2)
  </me>
  <men xml:id="eqn-KI1" >
   or, \quad \frac{b^2}{a^2} = 1-e^2
  </men>
  

  <men xml:id="eqn-newt18">
    \therefore \quad e = \sqrt{1-\frac{b^2}{a^2}}
  </men>
  
   
</p>
</proof>

</introduction>

<subsection xml:id="subsec-kepI">
  <title>Total Energy of Orbit</title>
  <p>
    Planetory orbits are closed so the total energy of orbit must be negative. Hence total energy,
    <me>
      E = KE+PE = \frac{1}{2}mv_{\theta}^2-\frac{GMm}{r}
    </me>
    along the orbit. Here <m>v^2=\dot{r}^2+r^2\dot{\theta}^2</m>
    <me>
      or, \quad E = \frac{1}{2}(\frac{mh^2}{r^2})-\frac{GMm}{r}
    </me>
    using <xref ref="eqn-polar4"/> and <xref ref="eqn-newt8"/>.
    <me>
      or, \quad E = \frac{1}{2}m(\frac{h}{r_{min}})^2 -\frac{GMm}{r_{min}}
    </me>
    at perihelion position. you may try from apehelion position energy.
  </p>
<p>
  <me>
E = \frac{1}{2}mh^2 (\frac{1+e}{l})^2 -\frac{GMm(1+e)}{l}
  </me>
<md>
  <mrow>or, E \amp =\frac{1}{2}mh^2 (\frac{G^2M^2m^4}{L^4})(1+e)^2 -\frac{G^2M^2m^3(1+e)}{L^2} </mrow>
  <mrow>or, E \amp = \frac{1}{2}\frac{G^2M^2m^3(1+e)^2}{L^2} -\frac{G^2M^2m^3(1+e)}{L^2}</mrow>
 </md>

 <men xml:id="eqn-newt19">
  \frac{1}{2}\alpha(1+e)^2 -\alpha(1+e)-E =0
 </men>
This is quadratic equation in (1+e). Here <m>\alpha = \frac{G^2M^2m^3}{L^2}</m>
<me>
  \therefore \quad 1+e = \frac{\alpha\pm\sqrt{\alpha^2+4\alpha/2 E}}{2\alpha/2}
</me>
Solving this equation, we get 
<me>
  E =-(1-e^2)\alpha/2 
</me>
Hence, E is negative for <m>0\lt e \lt 1.</m>
</p>

</subsection>


</section>